wip

HumanEvalLean/HumanEval129.lean
@@ -4,6 +4,8 @@ import Std
 import all Init.Data.Range.Polymorphic.RangeIterator
 open Std Std.Do
 
+set_option mvcgen.warning false
+
 def Vector.iter (xs : Vector α n) :=
     (xs.toArray.iter : Iter α)
 
@@ -33,7 +35,15 @@ instance [Iterator α Id β] [Iterators.Productive α Id] : Membership β (Iter 
 theorem Std.Iter.mem_toList_iff [Iterator α Id β] [Iterators.Finite α Id]
     {it : Iter (α := α) β} {x : β} :
     x ∈ it.toList ↔ x ∈ it := by
-  sorry
+  simp only [instMembershipIterOfProductiveId_humanEvalLean, List.mem_iff_getElem,
+    List.getElem_eq_getElem?_get, getElem?_toList_eq_atIdxSlow?]
+  apply Iff.intro
+  · rintro ⟨i, hi, rfl⟩
+    exact ⟨i, by grind⟩
+  · rintro ⟨i, h⟩
+    simp only [← getElem?_toList_eq_atIdxSlow?, Option.eq_some_iff_get_eq, get_getElem?,
+      isSome_getElem?] at h ⊢
+    exact ⟨i, h⟩
 
 theorem Std.Iter.atIdxSlow?_eq_getElem?_toList_take {α β} [Iterator α Id β] [Iterators.Productive α Id]
     {it : Iter (α := α) β} {k : Nat} :
@@ -90,13 +100,23 @@ theorem Std.Iter.mem_enumerate_iff [Iterator α Id β]
     atIdxSlow?_eq_getElem?_toList_take, Nat.toList_take_iter_rii, Nat.getElem?_toList_rio_eq_some_iff]
   grind
 
-theorem Vector.mem_iter_iff {xs : Vector α n} {x : α} :
-    x ∈ xs.iter ↔ x ∈ xs := by
-  sorry
+theorem Array.atIdxSlow?_iter {xs : Array α} {i : Nat} :
+    xs.iter.atIdxSlow? i = xs[i]? := by
+  grind [=_ Iter.getElem?_toList_eq_atIdxSlow?]
 
 theorem Vector.atIdxSlow?_iter {xs : Vector α n} {i : Nat} :
     xs.iter.atIdxSlow? i = xs[i]? := by
-  sorry
+  simp [Vector.iter, Array.atIdxSlow?_iter]
+
+theorem Array.mem_iter_iff {xs : Array α} {x : α} :
+    x ∈ xs.iter ↔ x ∈ xs := by
+  simp only [instMembershipIterOfProductiveId_humanEvalLean]
+  simp only [atIdxSlow?_iter, mem_iff_getElem]
+  grind
+
+theorem Vector.mem_iter_iff {xs : Vector α n} {x : α} :
+    x ∈ xs.iter ↔ x ∈ xs := by
+  simp [Vector.iter, Array.mem_iter_iff]
 
 theorem Vector.mem_enumerate_iter_iff {xs : Vector α n} {p : α × Nat} :
     p ∈ xs.iter.enumerate ↔ ∃ (h : p.2 < n), xs[p.2] = p.1 := by
@@ -143,6 +163,22 @@ def coordsOf? (grid : Vector (Vector Nat n) m) (l : Nat) : Option (Nat × Nat) :
     grid.iter.enumerate.findSome? (fun (row, x) =>
         row.iter.enumerate.findSome? (fun (cell, y) =>
             if cell = l then some (x, y) else none))
+
+theorem isSome_coordsOf? {grid : Vector (Vector Nat n) n} (h : WFGrid grid)
+    (hl : l ∈ 1...=(n * n)) :
+    (coordsOf? grid l).isSome := by
+  simp only [WFGrid] at h
+  simp only [coordsOf?, ← Iter.findSome?_toList, Iter.toList_enumerate, Vector.toList_iter]
+  simp only [List.isSome_findSome?]
+  have : l ∈ grid.flatten.toList := h.mem_iff.mpr (by simpa [Std.Rcc.mem_toList_iff_mem])
+  simp [Vector.flatten, Vector.toList_toArray] at this
+  obtain ⟨xs, ⟨⟨col, h_col_mem, heq⟩, h_l_mem⟩⟩ := this
+  simp only [Vector.mem_iff_getElem] at h_col_mem
+  obtain ⟨x, hx, hcol⟩ := h_col_mem
+  simp only [List.mem_iff_getElem] at h_l_mem
+  obtain ⟨y, hy, hcell⟩ := h_l_mem
+  simp only [List.any_eq_true, List.mem_zipIdx_iff_getElem?]
+  exact ⟨⟨col, x⟩, by grind, ⟨l, y⟩, by grind⟩
 
 theorem isSome_coordsOf?_one {grid : Vector (Vector Nat n) n} (hn : 0 < n) (h : WFGrid grid) :
     (coordsOf? grid 1).isSome := by
@@ -257,9 +293,6 @@ theorem AreNeighbors.down_of_pos {x y : Nat} (h : 0 < y) :
 
 attribute [grind .] AreNeighbors.right AreNeighbors.up
 
--- def IsInGrid (n : Nat) (p : Nat × Nat) : Prop :=
---     p.1 < n ∧ p.2 < n
-
 theorem exists_areNeighbors {p : Nat × Nat} (hn : 1 < n) (hxn : p.1 < n) (hyn : p.2 < n) :
     ∃ q, q.1 < n ∧ q.2 < n ∧ AreNeighbors p q := by
   by_cases hx : 0 < p.1
@@ -267,6 +300,22 @@ theorem exists_areNeighbors {p : Nat × Nat} (hn : 1 < n) (hxn : p.1 < n) (hyn :
     exact ⟨(p.1 - 1, p.2), by grind⟩
   · have := AreNeighbors.right (x := p.1) (y := p.2)
     exact ⟨(p.1 + 1, p.2), by grind⟩
+
+section Mathlib
+
+protected def Nat.findX {p : Nat → Prop}  (h : ∃ n, p n) : { n // p n ∧ ∀ m < n, ¬p m } := sorry
+protected def Nat.find {p : Nat → Prop} (h : ∃ n, p n) : Nat := (Nat.findX h).1
+protected theorem Nat.find_spec {p : Nat → Prop} (h : ∃ n, p n) : p (Nat.find h) :=
+  (Nat.findX h).2.left
+
+-- slightly deviates from mathlib's formulation
+protected theorem Nat.le_find_iff {p : Nat → Prop} (h : ∃ n, p n) {n : Nat} : n ≤ Nat.find h ↔ ∀ m, p m → n ≤ m := by
+  sorry
+
+protected theorem Nat.find_le {p : Nat → Prop} {h : ∃ n, p n} (hn : p n) : Nat.find h ≤ n :=
+  sorry
+
+end Mathlib
 
 theorem le_leastNeighborValue_iff {grid : Vector (Vector Nat n) n} {x y : Nat}
     (hn : 1 < n) (hg : WFGrid grid) (hx : x < n) (hy : y < n) :
@@ -291,10 +340,205 @@ theorem le_leastNeighborValue_iff {grid : Vector (Vector Nat n) n} {x y : Nat}
     have : k ≤ val₃ := by split at h₃ <;> (simp only [h₃, le_min_iff]; grind)
     split at h₄ <;> (simp only [h₄, le_min_iff]; grind)
 
+theorem exists_exists_areNeighbors {grid : Vector (Vector Nat n) n} (hn : 1 < n) (hx : x < n) (hy : y < n) :
+    ∃ (k x' y' : _) (_ : x' < n) (_ : y' < n), k = grid[x'][y'] ∧ AreNeighbors (x, y) (x', y') := by
+  obtain ⟨⟨x', y'⟩, hx', hy', hnb⟩ := exists_areNeighbors hn (p := (x, y)) hx hy
+  exact ⟨_, x', y', hx', hy', rfl, hnb⟩
+
+theorem leastNeighborValue_eq_natFind {grid : Vector (Vector Nat n) n} {x y : Nat}
+    (hn : 1 < n) (hg : WFGrid grid) (hx : x < n) (hy : y < n) :
+    leastNeighborValue grid x y = Nat.find (exists_exists_areNeighbors (grid := grid) hn hx hy) := by
+  apply le_antisymm
+  · simp only [Nat.le_find_iff]
+    grind [le_leastNeighborValue_iff]
+  · simp only [le_leastNeighborValue_iff hn hg hx hy]
+    intro x' y' hx' hy' hnb
+    apply Nat.find_le
+    grind
+
+theorem leastNeighborValue_mem_rcc {grid : Vector (Vector Nat n) n} {x y : Nat}
+    (hn : 1 < n) (hg : WFGrid grid) (hx : x < n) (hy : y < n) :
+    leastNeighborValue grid x y ∈ 1...=(n * n) := by
+  rw [leastNeighborValue_eq_natFind hn hg hx hy]
+  obtain ⟨x', y', hx', hy', h, hnb⟩ := Nat.find_spec (exists_exists_areNeighbors (grid := grid) hn hx hy)
+  rw [h, ← Std.Rcc.mem_toList_iff_mem]
+  apply hg.mem_iff.mp
+  simp only [Vector.mem_toList_iff, Vector.mem_flatten]
+  exact ⟨grid[x'], by grind⟩
+
+theorem leastNeighborValue_le {grid : Vector (Vector Nat n) n} {x y x' y' : Nat}
+    (hn : 1 < n) (hg : WFGrid grid) (hx : x < n) (hy : y < n) (hx' : x' < n) (hy' : y' < n)
+    (hnb : AreNeighbors (x, y) (x', y')) :
+    leastNeighborValue grid x y ≤ grid[x'][y'] := by
+  rw [leastNeighborValue_eq_natFind hn hg hx hy]
+  apply Nat.find_le
+  exact ⟨x', y', hx', hy', rfl, hnb⟩
+
+section Mathlib
+
+theorem List.Nodup.getElem_inj_iff {l : List α} (h : List.Nodup l)
+    {i : Nat} {hi : i < l.length} {j : Nat} {hj : j < l.length} :
+    l[i] = l[j] ↔ i = j := by
+  sorry
+
+end Mathlib
+
+public theorem Std.Rxc.Iterator.nodup_toList [LE α] [DecidableLE α]
+    [PRange.UpwardEnumerable α] [Rxc.IsAlwaysFinite α] [PRange.LawfulUpwardEnumerable α]
+    [PRange.LawfulUpwardEnumerableLE α]
+    {it : Iter (α := Rxc.Iterator α) α} :
+    it.toList.Nodup := by
+  apply (Rxc.Iterator.pairwise_toList_upwardEnumerableLt it).imp
+  grind [PRange.UpwardEnumerable.ne_of_lt]
+
+public theorem Std.Rcc.nodup_toList [LE α] [DecidableLE α]
+    [PRange.UpwardEnumerable α] [Rxc.IsAlwaysFinite α] [PRange.LawfulUpwardEnumerable α]
+    [PRange.LawfulUpwardEnumerableLE α]
+    {a b : α} :
+    (a...=b).toList.Nodup := by
+  grind [=_ Std.Rcc.toList_iter, Std.Rxc.Iterator.nodup_toList]
+
+theorem Vector.getElem_eq_getElem_toList {xs : Vector α n} {i : Nat} {hi : i < n} :
+    xs[i] = xs.toList[i]'(by grind) := by
+  simp
+
+theorem getElem_grid_inj {grid : Vector (Vector Nat n) n}
+    (hg : WFGrid grid) {p q : Nat × Nat} (hp : p.1 < n ∧ p.2 < n) (hq : q.1 < n ∧ q.2 < n)
+    (h : grid[p.1][p.2] = grid[q.1][q.2]) :
+    p = q := by
+  have hnodup : List.Nodup grid.flatten.toList := by
+    apply hg.nodup_iff.mpr
+    apply Std.Rcc.nodup_toList
+  suffices n * p.1 + p.2 = n * q.1 + q.2 by
+    ext
+    · have (p : Nat × Nat) (hp : p.1 < n ∧ p.2 < n) : p.1 = (n * p.1 + p.2) / n := by
+        simp only [Nat.mul_add_div (show 0 < n by grind)]
+        grind [Nat.div_eq_zero_iff]
+      grind
+    · have (p : Nat × Nat) (hp : p.1 < n ∧ p.2 < n) : p.2 = (n * p.1 + p.2) % n := by
+        simp [Nat.mod_eq_of_lt hp.2]
+      grind
+  have (p : Nat × Nat) (h : p.1 < n ∧ p.2 < n) : n * p.1 + p.2 < n * n := by
+    have : n * n = n * (n - 1) + n * 1 := by rw [← Nat.mul_add, Nat.sub_add_cancel (by grind)]
+    have : n * p.1 ≤ n * (n - 1) := Nat.mul_le_mul_left n (by grind)
+    grind
+  have (p : Nat × Nat) (h : p.1 < n ∧ p.2 < n) :
+      haveI := this p h; grid[p.fst][p.snd] = grid.flatten[n * p.fst + p.snd] := by
+    haveI := this p h
+    simp only [Vector.getElem_flatten, Nat.mul_add_mod_self_left, Nat.mod_eq_of_lt h.2]
+    have hn0 : 0 < n := by grind
+    simp only [Nat.mul_add_div hn0]
+    grind [Nat.div_eq_zero_iff]
+  rw [this p hp, this q hq] at h
+  simp only [Vector.getElem_eq_getElem_toList] at h
+  rwa [← hnodup.getElem_inj_iff]
+
+theorem getElem!_mem_rcc {grid : Vector (Vector Nat n) n} (hg : WFGrid grid) (hx : x < n) (hy : y < n) :
+    grid[x]![y]! ∈ 1...=(n * n) := by
+  simp only [← Std.Rcc.mem_toList_iff_mem]
+  apply hg.mem_iff.mp
+  simp only [Vector.mem_toList_iff]
+  apply Vector.mem_flatten_of_mem (xs := grid[x]) <;> grind
+
+theorem getElem_mem_rcc {grid : Vector (Vector Nat n) n} (hg : WFGrid grid) (hx : x < n) (hy : y < n) :
+    grid[x][y] ∈ 1...=(n * n) := by
+  have := getElem!_mem_rcc hg hx hy
+  grind
+
+theorem get!_coordsOf?_getElem {grid : Vector (Vector Nat n) n}
+    (hg : WFGrid grid) (hx : x < n) (hy : y < n) :
+    (coordsOf? grid grid[x][y]).get! = (x, y) := by
+  have hl : grid[x][y] ∈ 1...=(n * n) := by grind [getElem_mem_rcc]
+  have := isSome_coordsOf? hg hl
+  have := coordsOf?_spec (x := (coordsOf? grid grid[x][y]).get!.fst) (y := (coordsOf? grid grid[x][y]).get!.snd) (l := grid[x][y]) (grid := grid) (by simp only [Prod.eta, Option.some_get!, *])
+  apply getElem_grid_inj hg <;> grind
+
 theorem areNeighbors_coordsOf?_leastNeighborValue {grid : Vector (Vector Nat n) n} {p : Nat × Nat}
     (hn : 1 < n) (hg : WFGrid grid) (hx : p.1 < n) (hy : p.2 < n) :
     AreNeighbors p (coordsOf? grid (leastNeighborValue grid p.1 p.2)).get! := by
+  rw [leastNeighborValue_eq_natFind hn hg hx hy]
+  have := Nat.find_spec (exists_exists_areNeighbors (grid := grid) hn hx hy)
+  grind [get!_coordsOf?_getElem]
+
+theorem get_coordsOf?_bounds {grid : Vector (Vector Nat n) n} {l : Nat} {h} :
+    ((coordsOf? grid l).get h).fst < n ∧ ((coordsOf? grid l).get h).snd < n := by
+  have : coordsOf? grid l = some ((coordsOf? grid l).get!.fst, (coordsOf? grid l).get!.snd) := by grind [Option.some_get!]
+  grind [coordsOf?_spec]
+
+theorem get!_coordsOf?_bounds {grid : Vector (Vector Nat n) n} {l : Nat}
+    (hg : WFGrid grid) (hl : l ∈ 1...=(n * n)) :
+    (coordsOf? grid l).get!.fst < n ∧ (coordsOf? grid l).get!.snd < n := by
+  have := isSome_coordsOf? hg hl
+  have : coordsOf? grid l = some ((coordsOf? grid l).get!.fst, (coordsOf? grid l).get!.snd) := by grind [Option.some_get!]
+  grind [coordsOf?_spec]
+
+theorem getElem_minPath_mem_rcc {grid : Vector (Vector Nat n) n} {k : Nat} (hn : 1 < n)
+    (hg : WFGrid grid) {i : Nat} {h : i < (minPath grid k).length} :
+    (minPath grid k)[i]'h ∈ 1...=(n * n) := by
+  have : 1 < n * n := lt_of_lt_of_le hn (Nat.le_mul_self n)
+  by_cases i % 2 = 0
+  · rw [getElem_minPath_eq_one (by grind)]
+    grind [Std.Rcc.mem_iff]
+  · rw [getElem_minPath_of_odd hn hg (by grind)]
+    have (h : _) := get_coordsOf?_bounds (grid := grid) (l := 1) (h := h)
+    grind [leastNeighborValue_mem_rcc]
+
+theorem getElem_get!_coordsOf? {grid : Vector (Vector Nat n) n} {l : Nat} (hg : WFGrid grid)
+    (hl : l ∈ 1...=n * n) :
+    letI coords := (coordsOf? grid l).get!
+    haveI := get!_coordsOf?_bounds hg hl
+    grid[coords.1][coords.2] = l := by
+  have := isSome_coordsOf? hg hl
+  have : coordsOf? grid l = some ((coordsOf? grid l).get!.fst, (coordsOf? grid l).get!.snd) := by grind [Option.some_get!]
+  grind [coordsOf?_spec]
+
+theorem getElem!_get!_coordsOf? {grid : Vector (Vector Nat n) n} {l : Nat}
+    (hg : WFGrid grid) (hl : l ∈ 1...=n * n) :
+    letI coords := (coordsOf? grid l).get!
+    haveI := get!_coordsOf?_bounds hg hl
+    grid[coords.1]![coords.2]! = l := by
+  have := isSome_coordsOf? hg hl
+  have : coordsOf? grid l = some ((coordsOf? grid l).get!.fst, (coordsOf? grid l).get!.snd) := by grind [Option.some_get!]
+  grind [coordsOf?_spec]
+
+section Batteries
+
+/-- `IsChain R l` means that `R` holds between adjacent elements of `l`.
+```
+IsChain R [a, b, c, d] ↔ R a b ∧ R b c ∧ R c d
+``` -/
+inductive List.IsChain (R : α → α → Prop) : List α → Prop where
+  /-- A list of length 0 is a chain. -/
+  | nil : IsChain R []
+  /-- A list of length 1 is a chain. -/
+  | singleton (a : α) : IsChain R [a]
+  /-- If `a` relates to `b` and `b::l` is a chain, then `a :: b :: l` is also a chain. -/
+  | cons_cons (hr : R a b) (h : IsChain R (b :: l)) : IsChain R (a :: b :: l)
+
+
+theorem List.isChain_iff_getElem {l : List α} :
+    IsChain R l ↔ ∀ (i : Nat) (_hi : i + 1 < l.length), R l[i] l[i + 1] := by
   sorry
+
+theorem List.isChain_of_isChain_cons (p : List.IsChain R (b :: l)) :
+    List.IsChain R l := by
+  sorry
+
+end Batteries
+
+def minCoordPath (grid : Vector (Vector Nat n) n) (k : Nat) : List (Nat × Nat) :=
+    (minPath grid k).map (fun val => (coordsOf? grid val).get!)
+
+theorem map_getElem_minCoordPath {grid : Vector (Vector Nat n) n} {k : Nat}
+    (hn : 2 < n) (hg : WFGrid grid) :
+    (minCoordPath grid k).map (fun coord => grid[coord.1]![coord.2]!) = minPath grid k := by
+  simp only [minCoordPath, List.map_map]
+  apply List.ext_getElem
+  · grind
+  · simp
+    intro i hi _
+    rw [getElem!_get!_coordsOf? (n := n) (by grind)]
+    exact getElem_minPath_mem_rcc (by grind) hg
 
 theorem areNeighbors_minPath {grid : Vector (Vector Nat n) n} {k i : Nat}
     (hn : 1 < n) (hg : WFGrid grid) (hi : i + 1 < k) :
@@ -313,6 +557,71 @@ theorem areNeighbors_minPath {grid : Vector (Vector Nat n) n} {k i : Nat}
     simp only [Option.get_eq_get!]
     have := coordsOf?_spec (grid := grid) (l := 1) (x := (coordsOf? grid 1).get!.fst) (y := (coordsOf? grid 1).get!.snd) (Option.some_get! _ (isSome_coordsOf?_one (by grind) hg)).symm
     grind [areNeighbors_coordsOf?_leastNeighborValue, AreNeighbors.symm]
+
+theorem isChain_areNeighbors_minCoordPath {grid : Vector (Vector Nat n) n} {k : Nat}
+    (hn : 2 < n) (hg : WFGrid grid) :
+    (minCoordPath grid k).IsChain AreNeighbors := by
+  simp only [List.isChain_iff_getElem]
+  intro i hi
+  have := areNeighbors_minPath (n := n) (k := k) (i := i) (by grind) hg (by grind [length_minPath, minCoordPath])
+  simp only [minCoordPath, List.getElem_map]
+  grind
+
+theorem minPath_one {grid : Vector (Vector Nat n) n} (hn : 2 < n) (hg : WFGrid grid) :
+    minPath grid 1 = [1] := by
+  apply List.ext_getElem
+  · grind [length_minPath]
+  · grind [getElem_minPath_eq_one]
+
+theorem minPath_add_two {grid : Vector (Vector Nat n) n} (hn : 2 < n) (hg : WFGrid grid) :
+    let coords := (coordsOf? grid 1).get (isSome_coordsOf?_one (by grind) hg)
+    have := coordsOf?_spec (Option.some_get (isSome_coordsOf?_one (by grind) hg)).symm
+    let val := (leastNeighborValue grid coords.1 coords.2 (by grind))
+    minPath grid (k + 2) = 1 :: val :: minPath grid k := by
+  apply List.ext_getElem
+  · grind [length_minPath]
+  · intro i h₁ h₂
+    by_cases hi : i % 2 = 0
+    · grind [getElem_minPath_eq_one]
+    · grind [getElem_minPath_of_odd]
+
+theorem minPath_le_of_isChain_areNeighbors {grid : Vector (Vector Nat n) n} {k : Nat}
+    (hn : 2 < n) (hg : WFGrid grid) {cs : List (Nat × Nat)} (hcl : cs.length = k)
+    (hcb : ∀ c ∈ cs, c.1 < n ∧ c.2 < n)
+    (hcc : cs.IsChain AreNeighbors) :
+    (minPath grid k) ≤ cs.map (fun coord => grid[coord.1]![coord.2]!) := by
+  have := length_minPath (grid := grid) (k := k) (by grind) hg
+  match k with
+  | 0 => grind
+  | 1 =>
+    match cs with
+    | [] => grind
+    | [c] =>
+      specialize hcb c (List.mem_singleton_self _)
+      simp only [minPath_one hn hg, List.map_singleton, List.cons_le_cons_iff, List.nil_le, and_true]
+      have : grid[c.fst]![c.snd]! ∈ 1...=(n * n) := by grind [getElem!_mem_rcc]
+      grind [Std.Rcc.mem_iff]
+    | _ :: _ :: _ => grind
+  | k + 2 =>
+    match cs, hcc with
+    | [], _ | [_], _ => grind
+    | c₁ :: c₂ :: cs, .cons_cons hnb hcc =>
+      simp only [minPath_add_two hn hg, List.map_cons, List.cons_le_cons_iff]
+      have : grid[c₁.fst]![c₁.snd]! ∈ 1...=(n * n) := by grind [getElem!_mem_rcc]
+      by_cases 1 < grid[c₁.fst]![c₁.snd]!
+      · grind
+      · let coords := (coordsOf? grid 1).get!
+        have := coordsOf?_spec (grid := grid) (x := coords.1) (y := coords.2) (l := 1) (by grind [Option.some_get!, isSome_coordsOf?_one])
+        have : leastNeighborValue grid coords.1 coords.2 (by grind) ≤ grid[c₂.fst]![c₂.snd]! := by
+          rw [getElem!_pos (h := by grind), getElem!_pos (h := by grind)]
+          apply leastNeighborValue_le (by grind) hg (by grind) (by grind)
+          simp only [coords, Prod.eta]
+          have : c₁ = (coordsOf? grid 1).get! := by
+            apply getElem_grid_inj hg (by grind) (by grind)
+            grind [Std.Rcc.mem_iff]
+          grind
+        have := minPath_le_of_isChain_areNeighbors hn hg (k := k) (cs := cs)  (by grind) (by grind) (by grind [List.isChain_of_isChain_cons])
+        grind [Std.Rcc.mem_iff, Option.get_eq_get!]
 
 /-!
 ## Prompt
